ironfleet/ravana/DistributedSystem.i.dfy
@@ -1,0 +1,19 @@
+include "Node.i.dfy"
+include "Types.i.dfy"
+
+module DistributedSystem_i {
+  import opened Protocol_Node_i
+
+  predicate RS_Init(rs: RS_State, config: Config)
+  {
+       LEnvironment_Init(rs.environment)
+    && |config.node_controllers| > 0
+    && |config.node_switches| > 0
+    && NodeInit_Logger(config.node_logger, config)
+    && (forall e :: e in rs.servers <==> (e == config.node_logger
+          || e in config.node_controllers || e in config.node_switches))
+    && NodeInit_Controller(rs.servers[config.node_logger], config)
+    && (forall e in config.node_controllers ::
+          NodeInit_Logger
+  }
+}
